verified/ptables.i.dfy
@@ -1,24 +1,6 @@
 include "pagedb.i.dfy"
 include "entry.s.dfy"
 
-lemma UserExecutionMemInvariant(s:state, s':state, d:PageDb, l1:PageNr)
-    requires ValidState(s) && SaneMem(s.m)
-    requires evalUserspaceExecution(s, s')
-    requires validPageDb(d)
-    requires pageDbCorresponds(s.m, d)
-    requires nonStoppedL1(d, l1)
-    requires s.conf.ttbr0.ptbase == page_paddr(l1)
-    ensures WSMemInvariantExceptAddrspaceAtPage(s, s', d, l1)
-{
-    var l1pg := extractPage(s.m, l1);
-    var e := d[l1].entry;
-    assert e.L1PTable? && wellFormedPageDbEntryTyped(e);
-    assert pageContentsCorresponds(l1, d[l1], l1pg);
-    reveal_pageContentsCorresponds();
-    assert pageDbL1PTableCorresponds(l1, e, l1pg);
-    assume false;
-}
-
 function mkAbsPTE(pte: L2PTE): Maybe<AbsPTE>
     requires PhysBase() == KOM_DIRECTMAP_VBASE()
     ensures var r := mkAbsPTE(pte); r.Just? ==> WellformedAbsPTE(r.v)
@@ -38,7 +20,7 @@ function mkAbsPTE(pte: L2PTE): Maybe<AbsPTE>
     }
 }
 
-lemma {:axiom} l2ptesmatch(pte: L2PTE)
+lemma {:axiom} lemma_l2ptesmatch(pte: L2PTE)
     requires PhysBase() == KOM_DIRECTMAP_VBASE()
     ensures ExtractAbsL2PTE(mkL2Pte(pte)) == Just(mkAbsPTE(pte))
 /* FIXME: this is really gross right now (and contains several
@@ -81,6 +63,7 @@ lemma {:axiom} l2ptesmatch(pte: L2PTE)
     }
 } */
 
+/*
 function getAbsPTE(d:PageDb, l2:PageNr, i:int, j:int): Maybe<AbsPTE>
     requires validPageDb(d)
     requires validL2PTPage(d, l2) && !hasStoppedAddrspace(d, l2)
@@ -90,37 +73,7 @@ function getAbsPTE(d:PageDb, l2:PageNr, i:int, j:int): Maybe<AbsPTE>
 {
     mkAbsPTE(d[l2].entry.l2pt[i * 4 + j])
 }
-
-lemma lemma_memstatecontainspage(s:memstate, p:PageNr)
-    requires SaneMem(s)
-    ensures memContainsPage(s.addresses, p)
-{
-    var va := page_monvaddr(p);
-    assert ValidMemRange(va, va + PAGESIZE());
-    reveal_ValidMemState();
-}
-
-predicate l2tablesmatch(s:memstate, p:PageNr, e:PageDbEntryTyped)
-    requires PhysBase() == KOM_DIRECTMAP_VBASE()
-    requires ValidMemState(s)
-    requires e.L2PTable? && wellFormedPageDbEntryTyped(e)
-{
-    var vbase := page_monvaddr(p);
-    ValidMemRange(vbase, vbase + PAGESIZE())
-    && forall i | 0 <= i < 4 :: ExtractAbsL2PTable(s, vbase + i * ARM_L2PTABLE_BYTES(), 0)
-        == Just(mkAbsL2PTable(e, i))
-}
-
-lemma lemma_l2tablesmatch(s:memstate, p:PageNr, e:PageDbEntryTyped)
-    requires SaneMem(s)
-    requires PhysBase() == KOM_DIRECTMAP_VBASE()
-    requires e.L2PTable? && wellFormedPageDbEntryTyped(e)
-    requires pageDbL2PTableCorresponds(p, e, extractPage(s, p))
-    ensures l2tablesmatch(s, p, e)
-{
-    lemma_memstatecontainspage(s, p);
-    assume false; // TODO
-}
+*/
 
 function mkAbsL2PTable(e:PageDbEntryTyped, i:int): AbsL2PTable
     requires PhysBase() == KOM_DIRECTMAP_VBASE()
@@ -160,6 +113,80 @@ function mkAbsPTable'(d:PageDb, l1:PageNr, idx:int): AbsPTable
         first + mkAbsPTable'(d, l1, idx + 1)
 }
 
+lemma lemma_memstatecontainspage(s:memstate, p:PageNr)
+    requires SaneMem(s)
+    ensures memContainsPage(s.addresses, p)
+{
+    var va := page_monvaddr(p);
+    assert ValidMemRange(va, va + PAGESIZE());
+    reveal_ValidMemState();
+}
+
+predicate l2tablesmatch(s:memstate, p:PageNr, e:PageDbEntryTyped)
+    requires PhysBase() == KOM_DIRECTMAP_VBASE()
+    requires ValidMemState(s)
+    requires e.L2PTable? && wellFormedPageDbEntryTyped(e)
+{
+    var vbase := page_monvaddr(p);
+    ValidMemRange(vbase, vbase + PAGESIZE())
+    && forall i | 0 <= i < 4 :: ExtractAbsL2PTable(s, vbase + i * ARM_L2PTABLE_BYTES(), 0)
+        == Just(mkAbsL2PTable(e, i))
+}
+
+lemma lemma_ExtractAbsL2PTable(m:memstate, vbase:addr, i:nat)
+    requires ValidMemState(m)
+    requires WordAligned(vbase)
+        && ValidMemRange(vbase, vbase + ARM_L2PTABLE_BYTES())
+    requires 0 <= i <= ARM_L2PTES()
+    requires forall j | 0 <= j < ARM_L2PTES() :: ExtractAbsL2PTE(MemContents(m, vbase + WordsToBytes(j))).Just?
+    ensures ExtractAbsL2PTable(m, vbase, i).Just?
+    ensures forall j | 0 <= j < ARM_L2PTES() - i :: ExtractAbsL2PTable(m, vbase, i).v[j] == ExtractAbsL2PTE(MemContents(m, vbase + WordsToBytes(j+i))).v
+    decreases ARM_L2PTES() - i
+{
+    if (i != ARM_L2PTES()) {
+        var r := ExtractAbsL2PTable(m, vbase, i);
+        var rest := ExtractAbsL2PTable(m, vbase, i + 1);
+        var pte := ExtractAbsL2PTE(MemContents(m, vbase + WordsToBytes(i)));
+        assert pte.Just?;
+        lemma_ExtractAbsL2PTable(m, vbase, i + 1);
+        assert rest.Just?;
+        assert r == Just([fromJust(pte)] + fromJust(rest));
+    }
+}
+
+lemma lemma_l2tablesmatch(s:memstate, p:PageNr, e:PageDbEntryTyped)
+    requires SaneMem(s)
+    requires PhysBase() == KOM_DIRECTMAP_VBASE()
+    requires e.L2PTable? && wellFormedPageDbEntryTyped(e)
+    requires pageDbL2PTableCorresponds(p, e, extractPage(s, p))
+    ensures l2tablesmatch(s, p, e)
+{
+    var l2pt := e.l2pt;
+    var base := page_monvaddr(p);
+
+    assert ARM_L2PTES() * 4 == NR_L2PTES();
+    forall i, j | 0 <= i < 4 && 0 <= j < ARM_L2PTES()
+        ensures ExtractAbsL2PTE(MemContents(s, base + WordsToBytes(i * ARM_L2PTES() + j))) == Just(mkAbsPTE(l2pt[i * ARM_L2PTES() + j])) {
+        var idx := i * ARM_L2PTES() + j;
+        var pte := l2pt[idx];
+        lemma_memstatecontainspage(s, p);
+        reveal_pageDbL2PTableCorresponds();
+        assert MemContents(s, base + WordsToBytes(idx)) == mkL2Pte(pte);
+        assert i * ARM_L2PTABLE_BYTES() + WordsToBytes(j) == WordsToBytes(idx);
+        lemma_l2ptesmatch(pte);
+    }
+
+    forall i | 0 <= i < 4
+        ensures ExtractAbsL2PTable(s, base + i * ARM_L2PTABLE_BYTES(), 0)
+        == Just(mkAbsL2PTable(e, i)) {
+        assert forall j | 0 <= j < ARM_L2PTES() ::
+            mkAbsL2PTable(e, i)[j] == mkAbsPTE(l2pt[i * ARM_L2PTES() + j]) == ExtractAbsL2PTE(MemContents(s, base + i * ARM_L2PTABLE_BYTES() + WordsToBytes(j))).v;
+        lemma_ExtractAbsL2PTable(s, base + i * ARM_L2PTABLE_BYTES(), 0);
+        assert |mkAbsL2PTable(e, i)| == |ExtractAbsL2PTable(s, base + i * ARM_L2PTABLE_BYTES(), 0).v| == ARM_L2PTES();
+        assert forall j | 0 <= j < ARM_L2PTES() :: base + i * ARM_L2PTABLE_BYTES() + WordsToBytes(j) == base + WordsToBytes(j + i*ARM_L2PTES());
+    }
+}
+
 function mkAbsPTable(d:PageDb, l1:PageNr): AbsPTable
     requires PhysBase() == KOM_DIRECTMAP_VBASE()
     requires validPageDb(d)
@@ -167,4 +194,33 @@ function mkAbsPTable(d:PageDb, l1:PageNr): AbsPTable
     ensures WellformedAbsPTable(mkAbsPTable(d, l1))
 {
     mkAbsPTable'(d, l1, 0)
+}
+
+lemma lemma_ptablesmatch(s:memstate, d:PageDb, l1p:PageNr)
+    requires SaneMem(s)
+    requires PhysBase() == KOM_DIRECTMAP_VBASE()
+    requires validPageDb(d)
+    requires nonStoppedL1(d, l1p)
+    requires pageDbCorresponds(s, d)
+    ensures ExtractAbsL1PTable(s, page_monvaddr(l1p), 0) == Just(mkAbsPTable(d, l1p))
+{
+    assume false; // TODO
+}
+
+lemma UserExecutionMemInvariant(s:state, s':state, d:PageDb, l1:PageNr)
+    requires ValidState(s) && SaneMem(s.m)
+    requires evalUserspaceExecution(s, s')
+    requires validPageDb(d)
+    requires pageDbCorresponds(s.m, d)
+    requires nonStoppedL1(d, l1)
+    requires s.conf.ttbr0.ptbase == page_paddr(l1)
+    ensures WSMemInvariantExceptAddrspaceAtPage(s, s', d, l1)
+{
+    var l1pg := extractPage(s.m, l1);
+    var e := d[l1].entry;
+    assert e.L1PTable? && wellFormedPageDbEntryTyped(e);
+    assert pageContentsCorresponds(l1, d[l1], l1pg);
+    reveal_pageContentsCorresponds();
+    assert pageDbL1PTableCorresponds(l1, e, l1pg);
+    assume false; // TODO
 }
